proofs/xarrays/XArray16.ec
@@ -1,0 +1,48 @@
+(* -------------------------------------------------------------------- *)
+require import AllCore JWordExtra JArrayExtra CircuitBindings.
+require (*--*) Array16.
+
+from Jasmin require import JWord.
+
+(* -------------------------------------------------------------------- *)
+export Array16.Array16.
+
+(* -------------------------------------------------------------------- *)
+clone export PAE with
+      op size <- 16,
+  theory A    <- Array16.Array16.
+
+(* -------------------------------------------------------------------- *)
+clone BSA as BSA16 with
+      op size <- 16,
+  theory A    <- Array16.Array16
+
+  proof gt0_size by done.
+
+(* -------------------------------------------------------------------- *)
+clone BSWA as BSWA_16u8 with
+      op asize <- 16,
+      op bsize <- 8,
+  theory A     <- Array16.Array16,
+  theory BSA   <- BSA16,
+  theory W     <- W8 { rename "_XX" as "_8" },
+  theory WE    <- WE8,
+  theory BSW   <- BSW8
+  proof *.
+
+(* -------------------------------------------------------------------- *)
+clone BSWAS as BSWAS_16u8_128 with
+      op asize   <- 16,
+      op bsize   <- 8,
+      op ssize   <- 128,
+  theory A       <- Array16.Array16,
+  theory BSA     <- BSA16,
+  theory WB      <- W8  { rename "_XX" as "_8" },
+  theory WEB     <- WE8,
+  theory BSWB    <- BSW8,
+  theory WS      <- W128  { rename "_XX" as "_128" },
+  theory WES     <- WE128,
+  theory BSWS    <- BSW128,
+  theory BSWA    <- BSWA_16u8
+
+  proof le_size by done.
