proofs/xarrays/XArray256.ec
@@ -1,6 +1,7 @@
 (* -------------------------------------------------------------------- *)
 require import AllCore JWordExtra JArrayExtra CircuitBindings.
 require (*--*) Array256.
+require import XWords.
 
 from Jasmin require import JWord.
 
@@ -28,3 +29,31 @@ clone BSWA as BSWA_256u32 with
   theory W     <- W32 { rename "_XX" as "_32" },
   theory WE    <- WE32,
   theory BSW   <- BSW32.
+
+(* -------------------------------------------------------------------- *)
+clone BSWA as BSWA_256u13 with
+      op asize <- 256,
+      op bsize <- 13,
+  theory A     <- Array256.Array256,
+  theory BSA   <- BSA256,
+  theory W     <- W13 { rename "_XX" as "_13" },
+  theory WE    <- WE13,
+  theory BSW   <- BSW13.
+
+(* -------------------------------------------------------------------- *)
+clone BSWAS as BSWAS_256u32_256 with
+      op asize   <- 256,
+      op bsize   <- 32,
+      op ssize   <- 256,
+  theory A       <- Array256.Array256,
+  theory BSA     <- BSA256,
+  theory WB      <- W32  { rename "_XX" as "_32" },
+  theory WEB     <- WE32,
+  theory BSWB    <- BSW32,
+  theory WS      <- W256  { rename "_XX" as "_256" },
+  theory WES     <- WE256,
+  theory BSWS    <- BSW256,
+  theory BSWA    <- BSWA_256u32
+
+  proof le_size by done.
+  
