proofs/xarrays/XArray416.ec
@@ -1,0 +1,67 @@
+(* -------------------------------------------------------------------- *)
+require import AllCore JWordExtra JArrayExtra CircuitBindings.
+require (*--*) Array416.
+require import XWords JWordExtra.
+
+from Jasmin require import JWord.
+
+(* -------------------------------------------------------------------- *)
+require Array416.
+
+(* -------------------------------------------------------------------- *)
+clone export PAE with
+      op size <- 416,
+  theory A    <- Array416.Array416.
+
+(* -------------------------------------------------------------------- *)
+clone BSA as BSA416 with
+      op size <- 416,
+  theory A    <- Array416.Array416
+
+  proof gt0_size by done.
+
+(* -------------------------------------------------------------------- *)
+clone BSWA as BSWA_416u8 with
+      op asize <- 416,
+      op bsize <- 8,
+  theory A     <- Array416.Array416,
+  theory BSA   <- BSA416,
+  theory W     <- W8 { rename "_XX" as "_8" },
+  theory WE    <- WE8,
+  theory BSW   <- BSW8
+  proof *.
+
+(* -------------------------------------------------------------------- *)
+clone BSWAS as BSWAS_416u8_13 with
+      op asize   <- 416,
+      op bsize   <- 8,
+      op ssize   <- 13,
+  theory A       <- Array416.Array416,
+  theory BSA     <- BSA416,
+  theory WB      <- W8  { rename "_XX" as "_8" },
+  theory WEB     <- WE8,
+  theory BSWB    <- BSW8,
+  theory WS      <- W13  { rename "_XX" as "_13" },
+  theory WES     <- WE13,
+  theory BSWS    <- BSW13,
+  theory BSWA    <- BSWA_416u8
+
+  proof le_size by done.
+
+(* -------------------------------------------------------------------- *)
+clone BSWAS as BSWAS_416u8_128 with
+      op asize   <- 416,
+      op bsize   <- 8,
+      op ssize   <- 128,
+  theory A       <- Array416.Array416,
+  theory BSA     <- BSA416,
+  theory WB      <- W8  { rename "_XX" as "_8" },
+  theory WEB     <- WE8,
+  theory BSWB    <- BSW8,
+  theory WS      <- W128  { rename "_XX" as "_128" },
+  theory WES     <- WE128,
+  theory BSWS    <- BSW128,
+  theory BSWA    <- BSWA_416u8
+
+  proof le_size by done.
+  
