proofs/xwords/XWords.ec
@@ -1,0 +1,48 @@
+from Jasmin require import JWord.
+require import JWordExtra CircuitBindings.
+
+(* -------------------------------------------------------------------- *)
+
+clone BitWordSH as W13 with
+    op size <- 13
+    rename "_XX" as "_13"
+    proof gt0_size by done,
+          size_le_256 by done. export W13. export ALU.
+
+clone WE as WE13 with
+  op     size <- 13,
+  theory W    <- W13 { rename "_XX" as "_13" }.
+print WE13.
+  
+clone BSW as BSW13 with
+  op     size <- 13,
+  theory W    <- W13  { rename "_XX" as "_13" },
+  theory WE   <- WE13 { rename "_XX" as "_13" }.
+
+clone BS_WB_WS_U as BS_W32_W13_U with
+        op sizeS <- 13,
+        op sizeB <- 32,
+    theory WS    <- W13  { rename "_XX" as "_13"
+                           "'S" as "13"
+                           "'B" as "32"},
+    theory WSE   <- WE13 { rename "_XX" as "_13"
+                           "'S" as "13"
+                           "'B" as "32"},
+    theory WB    <- W32  { rename "_XX" as "_32"
+                           "'S" as "13"
+                           "'B" as "32"},
+    theory WBE   <- WE32 { rename "_XX" as "_32"
+                           "'S" as "13"
+                           "'B" as "32"},
+    theory BSWS  <- BSW13  { rename "_XX" as "_13"
+                                    "'S" as "13"
+                                    "'B" as "32" },
+    theory BSWB  <- BSW32  { rename "_XX" as "_32"
+                                    "'S" as "13"
+                                    "'B" as "32"}
+          rename "'S" as "13"
+          rename "'B" as "32"
+    proof *.
+
+    realize le_size by auto. 
+
